src/Rupicola/Examples/Cells/Cells.v
@@ -97,17 +97,17 @@ Section with_parameters.
     - repeat straightline; eauto.
   Qed.
 
-  #[global] Program Instance SimpleAllocable_cell : SimpleAllocable cell_value :=
-    {| ssize_in_bytes := Memory.bytes_per_word width;
-       ssize_in_bytes_mod := Z_mod_same_full _;
-       sP_to_bytes := _;
-       sP_from_bytes := _ |}.
+  #[global] Program Instance SimpleAllocable_cell : Allocable cell_value :=
+    {| size_in_bytes := Memory.bytes_per_word width;
+       size_in_bytes_mod := Z_mod_same_full _;
+       P_to_bytes := _;
+       P_from_bytes := _ |}.
   Next Obligation.
-    apply (sP_to_bytes (SimpleAllocable := SimpleAllocable_scalar)).
+    apply (P_to_bytes (Allocable := Allocable_scalar)).
   Qed.
   Next Obligation.
     intros m H.
-    edestruct (sP_from_bytes (SimpleAllocable := SimpleAllocable_scalar) _ _ H).
+    edestruct (P_from_bytes (Allocable := Allocable_scalar) _ _ H).
     exists {| data := x |}. assumption.
   Qed.
 End with_parameters.
